src/SDK/Serialize.dfy
@@ -89,23 +89,23 @@ module Serialize {
 
   // ----- SerializeAAD -----
 
-  method SerializeAAD(wr: Streams.ByteWriter, kvPairs: EncryptionContext.T) returns (ret: Result<nat>)
-    requires wr.Valid() && EncryptionContext.ValidAAD(kvPairs)
+  method SerializeAAD(wr: Streams.ByteWriter, kvPairs: EncryptionContext.Map) returns (ret: Result<nat>)
+    requires wr.Valid() && EncryptionContext.Valid(kvPairs)
     modifies wr.writer`data
-    ensures wr.Valid() && EncryptionContext.ValidAAD(kvPairs)
+    ensures wr.Valid() && EncryptionContext.Valid(kvPairs)
     ensures match ret
       case Success(totalWritten) =>
-        var serAAD := EncryptionContext.AADToSeq(kvPairs);
+        var serAAD := EncryptionContext.MapToLinear(kvPairs);
         var initLen := old(wr.GetSizeWritten());
         && totalWritten == |serAAD|
         && initLen + totalWritten == wr.GetSizeWritten()
         && wr.GetDataWritten() == old(wr.GetDataWritten()) + serAAD
       case Failure(e) => true
   {
-    reveal EncryptionContext.ValidAAD();
+    reveal EncryptionContext.Valid();
     var totalWritten := 0;
 
-    var kvPairsLength := EncryptionContext.ComputeKVPairsLength(kvPairs);
+    var kvPairsLength := EncryptionContext.ComputeLength(kvPairs);
     var len := wr.WriteUInt16(kvPairsLength as uint16);
 
     totalWritten := totalWritten + len;
@@ -118,13 +118,13 @@ module Serialize {
 
   // ----- SerializeKVPairs -----
 
-  method SerializeKVPairs(wr: Streams.ByteWriter, encryptionContext: EncryptionContext.T) returns (ret: Result<nat>)
+  method SerializeKVPairs(wr: Streams.ByteWriter, encryptionContext: EncryptionContext.Map) returns (ret: Result<nat>)
     requires wr.Valid() && EncryptionContext.ValidKVPairs(encryptionContext)
     modifies wr.writer`data
     ensures wr.Valid() && EncryptionContext.ValidKVPairs(encryptionContext)
     ensures match ret
       case Success(totalWritten) =>
-        var serAAD := EncryptionContext.KVPairsToSeq(encryptionContext);
+        var serAAD := EncryptionContext.MapToSeq(encryptionContext);
         var initLen := old(wr.GetSizeWritten());
         && totalWritten == |serAAD|
         && initLen + totalWritten == wr.GetSizeWritten()
@@ -152,8 +152,8 @@ module Serialize {
       invariant wr.GetDataWritten() ==
         old(wr.GetDataWritten()) +
         UInt16ToSeq(n as uint16) +
-        EncryptionContext.KVPairEntriesToSeq(kvPairs, 0, j)
-      invariant totalWritten == 2 + |EncryptionContext.KVPairEntriesToSeq(kvPairs, 0, j)|
+        EncryptionContext.LinearToSeq(kvPairs, 0, j)
+      invariant totalWritten == 2 + |EncryptionContext.LinearToSeq(kvPairs, 0, j)|
     {
       ghost var previouslyWritten := wr.GetDataWritten();
 
@@ -174,11 +174,11 @@ module Serialize {
       ==  // the four writes in this loop iteration write EncryptionContext.KVPairToSeq(kvPairs[j])
         previouslyWritten + EncryptionContext.KVPairToSeq(kvPairs[j]);
       ==  // loop invariant on entry to loop
-        (old(wr.GetDataWritten()) + UInt16ToSeq(n as uint16) + EncryptionContext.KVPairEntriesToSeq(kvPairs, 0, j)) + EncryptionContext.KVPairToSeq(kvPairs[j]);
+        (old(wr.GetDataWritten()) + UInt16ToSeq(n as uint16) + EncryptionContext.LinearToSeq(kvPairs, 0, j)) + EncryptionContext.KVPairToSeq(kvPairs[j]);
       ==  // + is associative
-        old(wr.GetDataWritten()) + UInt16ToSeq(n as uint16) + (EncryptionContext.KVPairEntriesToSeq(kvPairs, 0, j) + EncryptionContext.KVPairToSeq(kvPairs[j]));
-      ==  { assert EncryptionContext.KVPairEntriesToSeq(kvPairs, 0, j) + EncryptionContext.KVPairToSeq(kvPairs[j]) == EncryptionContext.KVPairEntriesToSeq(kvPairs, 0, j + 1); }
-        old(wr.GetDataWritten()) + UInt16ToSeq(n as uint16) + EncryptionContext.KVPairEntriesToSeq(kvPairs, 0, j + 1);
+        old(wr.GetDataWritten()) + UInt16ToSeq(n as uint16) + (EncryptionContext.LinearToSeq(kvPairs, 0, j) + EncryptionContext.KVPairToSeq(kvPairs[j]));
+      ==  { assert EncryptionContext.LinearToSeq(kvPairs, 0, j) + EncryptionContext.KVPairToSeq(kvPairs[j]) == EncryptionContext.LinearToSeq(kvPairs, 0, j + 1); }
+        old(wr.GetDataWritten()) + UInt16ToSeq(n as uint16) + EncryptionContext.LinearToSeq(kvPairs, 0, j + 1);
       }
 
       j := j + 1;
